\section{Introducción}

El método de Stokes consiste en

\begin{equation}
    \label{eq:newton}
    m_b\,\frac{d^2 z}{dt^2} = - m_b\, g + m\,g - 6\,\pi\,\eta\,r\,\frac{dz}{dt}
\end{equation}


\begin{align}
    \label{eq:solution}
    z(t) &= z_0 + \beta \, (1 - e^{-\alpha t} -\alpha \,t) \\
    v(t) &= - \alpha \, \beta \, (1 - e^{-\alpha t})
\end{align}

\begin{align*}
    \alpha &= \frac{9}{2} \, \frac{\eta}{r^2\,\rho_b} \\
    \beta &= \biggl(  1 - \frac{\rho}{\rho_b} \biggr)\, \frac{g}{\alpha^2}  \\
\end{align*}

\begin{equation}
    \label{eq:velocity}
    v = - \alpha \, \beta = - \frac{2}{9} \, \biggl(1 - \frac{\rho}{\rho_b} \biggr) \, g \, \frac{\rho_b}{\eta} \, r^2
\end{equation}

\begin{equation}
    \label{eq:viscosity}
    \eta = - \frac{2}{9} \, \biggl(1 - \frac{\rho}{\rho_b} \biggr) \, g \, \frac{\rho_b}{v} \, r^2
\end{equation}



